---
layout: post
title: Proving Trig Identities
created: 1328713211
---
$$1) \sec t - \tan x \sin x = \frac{1}{\sec x}$$
$$\frac{1}{\cos t}-\frac{\sin t}{\cos t}\frac{\sin t}{1}=$$
$$\frac{1}{\cos t}-\frac{\sin^2 t}{\cos t}=$$
$$\frac{1}{\cos t}-\frac{\sin^2 t}{\cos t}=$$
$$\frac{1 - \sin^2 t}{\cos t}=$$
$$\frac{\cos^2 t}{\cos t}=\cos t = \frac{1}{\sec x}$$
<br /><br />
$$2) \frac{1+ \cos t}{\sin t} = \csc t + \cot t$$
$$ \frac{1}{\sin t} + \frac{\cos t}{\sin t} \Rightarrow \csc t + \cot t$$
<br /><br />
$$3) \frac{\tan t}{\sec t} + \frac{\cot t}{\csc t}=\sin t + \cos t$$
$$\frac{\sin t}{\cos t} \frac{1}{\sec t}+\frac{\cos t}{\sin t}\frac{1}{\csc t}=$$
$$\frac{\sin t}{\cos t} \frac{\cos t}{1}+\frac{\cos t}{\sin t}\frac{\sin t}{1}=$$
$$\sin t + \cos t$$
<br /><br />
$$4) \csc^2 t \cdot \tan^2 t -1 = \tan^2 t$$
$$\frac{1}{\sin^2t}\cdot \frac{\sin^2 t}{\cos^2 t} -1 = $$
$$\frac{1}{cos^2 t} -1 = $$
$$\sec^2 t -1 = \tan^2 t$$
<br /><br />
$$5)\cos t (\csc t + \tan t)=\cot t + \sin t$$
$$\cos t \cdot \frac{1}{\sin t} + \cos t \cdot \frac{\sin t}{\cos t}=$$
$$\tan t + \sin t $$
